Proofs/SHA512/Sha512.lean
@@ -1,3 +1,3 @@
 import Proofs.SHA512.Sha512_block_armv8_rules
 import Proofs.SHA512.Sha512_block_armv8
-import Proofs.SHA512.Sha512_Decode
+import Proofs.SHA512.Sha512Sym
