Proofs/SHA512/Sha512FetchLemmas.lean
@@ -5,6 +5,6 @@ import Proofs.SHA512.Sha512Program
 -- set_option trace.gen_step.debug.heartBeats true in
 set_option trace.gen_step.print_names true in
 set_option maxHeartbeats 1000000 in
-#genStepTheorems sha512_program namePrefix:="sha512_" thmType:="fetch" simpExt:=`state_simp_rules
+#genStepTheorems sha512_program namePrefix:="sha512_" thmType:="fetch"
 
 #check sha512_fetch_0x1264e8
