Proofs/SHA512/Sha512StepLemmas.lean
@@ -6,6 +6,6 @@ import Proofs.SHA512.Sha512Program
 -- set_option trace.gen_step.debug.heartBeats true in
 set_option trace.gen_step.print_names true in
 set_option maxHeartbeats 2000000 in
-#genStepTheorems sha512_program namePrefix:="sha512_" thmType:="step" simpExt:=`state_simp_rules
+#genStepTheorems sha512_program namePrefix:="sha512_" thmType:="step" `state_simp_rules
 
 #check sha512_stepi_0x1264e8
